encountered type error in Impl

concurrency/framework/AsyncSSM.s.dfy
@@ -104,3 +104,154 @@ module Obligations(
        )
   )
 { }
+
+module TicketStubPCM(IOIfc: InputOutputIfc,
+  ssm: TicketStubSSM(IOIfc)) refines PCM {
+  
+  type M = ssm.M
+
+  function dot(x: M, y: M) : M
+  {
+    ssm.dot(x, y)
+  }
+
+  predicate valid(x: M)
+  {
+    exists y: M :: ssm.Inv(dot(x, y))
+  }
+
+  function unit(): M
+  {
+    ssm.unit()
+  }
+
+  lemma dot_unit(x: M)
+  {
+    ssm.dot_unit(x);
+  }
+
+  lemma valid_unit(x: M)
+  {
+    var x := ssm.exists_inv_state();
+    commutative(unit(), x);
+    dot_unit(x);
+    assert ssm.Inv(dot(unit(), x));
+  }
+
+  lemma commutative(x: M, y: M)
+  //ensures dot(x, y) == dot(y, x)
+  {
+    ssm.commutative(x, y);
+  }
+
+  lemma associative(x: M, y: M, z: M)
+  //ensures dot(x, dot(y, z)) == dot(dot(x, y), z)
+  {
+    ssm.associative(x, y, z);
+  }
+
+  predicate single_step_helper(a: M, b: M, a': M, b': M, c: M) {
+    a == dot(a', c) && b == dot(b', c) && ssm.Internal(a', b')
+  }
+
+  predicate single_step(a: M, b: M) {
+    exists a', b', c :: single_step_helper(a, b, a', b', c)
+  }
+
+  least predicate reachable(a: M, b: M) {
+    a == b || (exists z :: reachable(a, z) && single_step(z, b))
+  }
+
+  predicate transition(a: M, b: M) {
+    reachable(a, b)
+  }
+
+  lemma transition_is_refl(a: M)
+  //requires transition(a, a)
+  {
+  }
+
+  least lemma reachable_is_trans(a: M, b: M, c: M)
+  requires reachable(b, c)
+  requires transition(a, b)
+  ensures reachable(a, c)
+  {
+    if b == c {
+    } else {
+      var z :| reachable(b, z) && single_step(z, c);
+      reachable_is_trans(a, b, z);
+    }
+  }
+
+  lemma transition_is_trans(a: M, b: M, c: M)
+  //requires transition(a, b)
+  //requires transition(b, c)
+  ensures transition(a, c)
+  {
+    reachable_is_trans(a, b, c);
+  }
+
+  least lemma reachable_is_monotonic(a: M, b: M, c: M)
+  requires reachable(a, b)
+  ensures reachable(dot(a, c), dot(b, c))
+  {
+    if a == b {
+    } else {
+      var z :| reachable(a, z) && single_step(z, b);
+      reachable_is_monotonic(a, z, c);
+      var z', b', d :| single_step_helper(z, b, z', b', d);
+      associative(z', d, c);
+      associative(b', d, c);
+      assert single_step_helper(dot(z, c), dot(b, c), z', b', dot(d, c));
+      assert single_step(dot(z, c), dot(b, c));
+    }
+  }
+
+  lemma transition_is_monotonic(a: M, b: M, c: M)
+  //requires transition(a, b)
+  ensures transition(dot(a, c), dot(b, c))
+  {
+    reachable_is_monotonic(a, b, c);
+  }
+}
+
+module TicketStubToken(IOIfc: InputOutputIfc,
+  ssm: TicketStubSSM(IOIfc)) {
+  import pcm = TicketStubPCM(IOIfc, ssm)
+  import Tokens = Tokens(pcm)
+
+  type Token = Tokens.Token
+
+  lemma transition_of_next(a: ssm.M, b: ssm.M)
+  requires ssm.Internal(a, b)
+  ensures pcm.transition(a, b)
+  {
+    ssm.dot_unit(a);
+    ssm.dot_unit(b);
+    var a' := a;
+    var b' := b;
+    var c := ssm.unit();
+    assert a == ssm.dot(a', c) && b == ssm.dot(b', c) && ssm.Internal(a', b');
+    assert pcm.single_step_helper(a, b, a', b', c);
+    assert pcm.single_step(a, b);
+  }
+
+  lemma transition_of_next_with_unit(a: ssm.M, b: ssm.M)
+  requires ssm.Internal(a, b)
+  ensures pcm.transition(pcm.dot(ssm.unit(), a), pcm.dot(ssm.unit(), b))
+  {
+    ssm.dot_unit(a);
+    ssm.dot_unit(b);
+    ssm.commutative(a, ssm.unit());
+    ssm.commutative(b, ssm.unit());
+    transition_of_next(a, b);
+  }
+
+  function method {:opaque} update_next(glinear a: Token, ghost expect_b: ssm.M): (glinear b: Token)
+  requires ssm.Internal(a.val, expect_b)
+  ensures b == Tokens.Token(a.loc, expect_b)
+  {
+    transition_of_next_with_unit(a.val, expect_b);
+    Tokens.transition_update(Tokens.get_unit_shared(a.loc), a, expect_b)
+  }
+}
