concurrency/framework/GhostLinearMaybe.s.dfy
@@ -1,0 +1,39 @@
+
+module GhostLinearMaybe {
+  // note: cannot test gmaybe<A> for equality at run-time (because has is ghost)
+  type {:extern "predefined"} gmaybe(!new)<A>
+
+  predicate {:axiom} has<A>(m: gmaybe<A>)
+
+  // return value in m if has(m), return default ghost A value otherwise
+  function {:axiom} read<A>(m: gmaybe<A>): A
+
+  function method peek<A>(gshared m: gmaybe<A>): (gshared a: A)
+    requires has(m)
+    ensures a == read(m)
+
+  function method unwrap<A>(glinear m: gmaybe<A>): (glinear a: A)
+    requires has(m)
+    ensures a == read(m)
+
+  function method give<A>(glinear a: A):(glinear m: gmaybe<A>)
+    ensures has(m)
+    ensures read(m) == a
+    ensures forall x:gmaybe<A> {:trigger give(read(x))} | has(x) && a == read(x) :: m == x
+
+  function method empty<A>():(glinear m: gmaybe<A>)
+    ensures !has(m)
+
+  function method discard<A>(glinear m:gmaybe<A>):()
+    requires !has(m)
+
+  // function {:axiom} imagine<A>(h:bool, a:A):(m:gmaybe<A>)
+  //   ensures has(m) == h
+  //   ensures read(m) == a
+
+  // lemma {:axiom} axiom_extensional<A>(m1:gmaybe<A>, m2:gmaybe<A>)
+  //   requires has(m1) == has(m2)
+  //   requires read(m1) == read(m2)
+  //   ensures m1 == m2
+
+} // module
